src/Formalization/Pipeline/Compiler_Correctness_Prototype.thy
@@ -134,6 +134,55 @@ proof -
     using eq first second unfolding compile_endpoints_def by simp
 qed
 
+fun endpoint_view :: "proc_info option \<Rightarrow> (pp \<times> pp) option"
+where
+  "endpoint_view None = None"
+| "endpoint_view (Some (en, ex, Ns, E, C)) = Some (en, ex)"
+
+definition layouts_agree :: "proc_layout \<Rightarrow> proc_layout \<Rightarrow> bool"
+where
+  "layouts_agree lay1 lay2 \<longleftrightarrow>
+    (\<forall>p. endpoint_view (lay1 p) = endpoint_view (lay2 p))"
+
+lemma compile_layouts_agree:
+  assumes agree: "layouts_agree lay1 lay2"
+  shows "compile Pi lay1 cmd n = compile Pi lay2 cmd n"
+  using agree
+proof (induction cmd arbitrary: n)
+  case SKIP
+  show ?case by simp
+next
+  case Assign
+  show ?case by simp
+next
+  case (Seq c1 c2)
+  show ?case
+    by (simp add: Seq.IH(1)[OF Seq.prems] Seq.IH(2)[OF Seq.prems])
+next
+  case If
+  show ?case
+    by (simp add: If.IH(1)[OF If.prems] If.IH(2)[OF If.prems])
+next
+  case While
+  show ?case
+    by (simp add: While.IH[OF While.prems])
+next
+  case Scope
+  show ?case
+    by (simp add: Scope.IH[OF Scope.prems])
+next
+  case (Call p)
+  have view: "endpoint_view (lay1 p) = endpoint_view (lay2 p)"
+    using Call.prems unfolding layouts_agree_def by blast
+  show ?case
+    using view
+    by (cases "lay1 p"; cases "lay2 p")
+       (auto split: prod.splits)
+next
+  case Restore
+  show ?case by simp
+qed
+
 lemma compile_procs_layout_domain:
   assumes distinct: "distinct ps"
       and fresh: "\<forall>p \<in> set ps. lay p = None"
@@ -184,7 +233,7 @@ lemma compile_procs_layout_domain_exact:
   by (auto simp: wf_compile_input_def layout_domain_exact_def)
 
 lemma compile_procs_layout_preserves:
-  assumes result: "compile_procs_layout \<Pi> ps lay n = (n', lay')"
+  assumes result: "compile_procs_layout Pi ps lay n = (n', lay')"
       and present: "lay p = Some info"
   shows "lay' p = Some info"
   using result present
@@ -194,9 +243,9 @@ proof (induction ps arbitrary: lay n n' lay')
 next
   case (Cons a ps)
   show ?case
-  proof (cases "\<Pi> a")
+  proof (cases "Pi a")
     case None
-    have rec: "compile_procs_layout \<Pi> ps lay n = (n', lay')"
+    have rec: "compile_procs_layout Pi ps lay n = (n', lay')"
       using Cons.prems(1) None by simp
     show ?thesis
       by (rule Cons.IH[OF rec Cons.prems(2)])
@@ -204,16 +253,16 @@ next
     case (Some cmd)
     note proc = Some
     obtain k en ex E C where comp:
-        "compile \<Pi> (known_proc_layout \<Pi> (a # ps) lay) cmd n =
+        "compile Pi (known_proc_layout Pi (a # ps) lay) cmd n =
           (k, en, ex, E, C)"
-      by (cases "compile \<Pi> (known_proc_layout \<Pi> (a # ps) lay) cmd n")
+      by (cases "compile Pi (known_proc_layout Pi (a # ps) lay) cmd n")
          auto
     show ?thesis
     proof (cases "lay a")
       case None
       note absent = None
       have rec:
-          "compile_procs_layout \<Pi> ps
+          "compile_procs_layout Pi ps
             (lay(a := Some (en, ex, {n..<k}, {}, {}))) k =
             (n', lay')"
         using Cons.prems(1) proc comp absent by simp
@@ -227,11 +276,62 @@ next
     next
       case (Some current)
       note present_a = Some
-      have rec: "compile_procs_layout \<Pi> ps lay k = (n', lay')"
+      have rec: "compile_procs_layout Pi ps lay k = (n', lay')"
         using Cons.prems(1) proc comp present_a by simp
       show ?thesis
         by (rule Cons.IH[OF rec Cons.prems(2)])
     qed
+  qed
+qed
+
+lemma compile_procs_layout_member:
+  assumes distinct: "distinct ps"
+      and fresh: "\<forall>q \<in> set ps. in_lay q = None"
+      and defined: "\<forall>q \<in> set ps. Pi q \<noteq> None"
+      and result:
+        "compile_procs_layout Pi ps in_lay n = (n', out_lay)"
+      and member: "p \<in> set ps"
+  shows "\<exists>en ex Ns.
+    out_lay p = Some (en, ex, Ns, {}, {})"
+  using distinct fresh defined result member
+proof (induction ps arbitrary: in_lay n n' out_lay p)
+  case Nil
+  then show ?case by simp
+next
+  case (Cons a ps)
+  obtain head_cmd where head: "Pi a = Some head_cmd"
+    using Cons.prems(3) by auto
+  obtain k head_en head_ex head_E head_C where comp:
+      "compile Pi (known_proc_layout Pi (a # ps) in_lay)
+        head_cmd n =
+        (k, head_en, head_ex, head_E, head_C)"
+    by (cases "compile Pi
+      (known_proc_layout Pi (a # ps) in_lay) head_cmd n") auto
+  define next_lay where
+    "next_lay =
+      in_lay(a := Some (head_en, head_ex, {n..<k}, {}, {}))"
+  have rec:
+      "compile_procs_layout Pi ps next_lay k = (n', out_lay)"
+    using Cons.prems(4) head comp Cons.prems(2)
+    by (simp add: next_lay_def)
+  show ?case
+  proof (cases "p = a")
+    case True
+    have stored:
+        "out_lay a =
+          Some (head_en, head_ex, {n..<k}, {}, {})"
+      by (rule compile_procs_layout_preserves[OF rec])
+         (simp add: next_lay_def)
+    then show ?thesis
+      using True by blast
+  next
+    case False
+    have fresh_tail: "\<forall>q \<in> set ps. next_lay q = None"
+      using Cons.prems(1,2)
+      by (auto simp: next_lay_def)
+    show ?thesis
+      by (rule Cons.IH[OF _ fresh_tail _ rec])
+         (use Cons.prems False in auto)
   qed
 qed
 
@@ -290,6 +390,90 @@ next
     qed
   qed
 qed
+
+lemma compile_procs_bodies_lookup:
+  assumes distinct: "distinct ps"
+      and fresh: "\<forall>q \<in> set ps. in_lay q = None"
+      and bodies:
+        "compile_procs_bodies Pi ps base_lay in_lay n =
+          (n', out_lay, E, C)"
+      and member: "p \<in> set ps"
+      and body: "Pi p = Some cmd"
+      and lookup:
+        "out_lay p = Some (en, ex, Ns, Ep, Cp)"
+  shows "\<exists>start finish.
+    compile Pi base_lay cmd start = (finish, en, ex, Ep, Cp)"
+  using distinct fresh bodies member body lookup
+proof (induction ps arbitrary: in_lay n n' out_lay E C p cmd
+    en ex Ns Ep Cp)
+  case Nil
+  then show ?case by simp
+next
+  case (Cons a ps)
+  show ?case
+  proof (cases "Pi a")
+    case None
+    have neq: "p \<noteq> a"
+      using Cons.prems(5) None by auto
+    have rec:
+        "compile_procs_bodies Pi ps base_lay in_lay n =
+          (n', out_lay, E, C)"
+      using Cons.prems(3) None by simp
+    show ?thesis
+      by (rule Cons.IH[OF _ _ rec])
+         (use Cons.prems neq in auto)
+  next
+    case (Some head_cmd)
+    note head = Some
+    obtain k head_en head_ex head_E head_C where comp:
+        "compile Pi base_lay head_cmd n =
+          (k, head_en, head_ex, head_E, head_C)"
+      by (cases "compile Pi base_lay head_cmd n") auto
+    define next_lay where
+      "next_lay =
+        in_lay(a := Some
+          (head_en, head_ex, {n..<k}, head_E, head_C))"
+    have absent: "in_lay a = None"
+      using Cons.prems(2) by simp
+    obtain Erest Crest where rec:
+        "compile_procs_bodies Pi ps base_lay next_lay k =
+          (n', out_lay, Erest, Crest)"
+      using Cons.prems(3) head comp absent
+      by (auto simp: next_lay_def split: prod.splits)
+    show ?thesis
+    proof (cases "p = a")
+      case True
+      have stored:
+          "out_lay a = Some
+            (head_en, head_ex, {n..<k}, head_E, head_C)"
+        by (rule compile_procs_bodies_preserves[OF rec])
+           (simp add: next_lay_def)
+      have cmd_eq: "cmd = head_cmd"
+        using Cons.prems(5) head True by simp
+      show ?thesis
+        using comp Cons.prems(6) stored True cmd_eq by auto
+    next
+      case False
+      have fresh_tail: "\<forall>q \<in> set ps. next_lay q = None"
+        using Cons.prems(1,2)
+        by (auto simp: next_lay_def)
+      show ?thesis
+        by (rule Cons.IH[OF _ fresh_tail rec])
+           (use Cons.prems False in auto)
+    qed
+  qed
+qed
+
+lemma compile_procs_bodies_outside:
+  assumes result:
+    "compile_procs_bodies Pi ps base_lay in_lay n =
+      (n', out_lay, E, C)"
+      and outside: "p \<notin> set ps"
+      and absent: "in_lay p = None"
+  shows "out_lay p = None"
+  using result outside absent
+  by (induction ps arbitrary: in_lay n n' out_lay E C)
+     (auto split: option.splits prod.splits)
 
 lemma compile_procs_pass_endpoint_agreement_general:
   assumes distinct: "distinct ps"
@@ -408,6 +592,81 @@ lemma compile_procs_pass_endpoint_agreement:
       using wf by (auto simp: wf_compile_input_def)
   qed
 
+lemma compile_procs_pass_layouts_agree:
+  assumes wf: "wf_compile_input Pi ps main"
+      and layout:
+        "compile_procs_layout Pi ps (\<lambda>_. None) 0 =
+          (n, base_lay)"
+      and bodies:
+        "compile_procs_bodies Pi ps base_lay (\<lambda>_. None) 0 =
+          (n', full_lay, E, C)"
+  shows "layouts_agree base_lay full_lay"
+proof (unfold layouts_agree_def, intro allI)
+  fix p
+  show "endpoint_view (base_lay p) = endpoint_view (full_lay p)"
+  proof (cases "p \<in> set ps")
+    case True
+    obtain cmd where body: "Pi p = Some cmd"
+      using wf True
+      by (auto simp: wf_compile_input_def)
+    have distinct: "distinct ps"
+      using wf by (auto simp: wf_compile_input_def)
+    have defined: "\<forall>q\<in>set ps. Pi q \<noteq> None"
+      using wf by (auto simp: wf_compile_input_def)
+    have member_info:
+        "\<exists>en ex Ns. base_lay p = Some (en, ex, Ns, {}, {})"
+      by (rule compile_procs_layout_member[
+            OF distinct _ defined layout True])
+         simp
+    then obtain en ex Ns where base:
+        "base_lay p = Some (en, ex, Ns, {}, {})"
+      by blast
+    obtain Ns' Ep Cp where full:
+        "full_lay p = Some (en, ex, Ns', Ep, Cp)"
+      using compile_procs_pass_endpoint_agreement[
+        OF wf layout bodies True body base] by blast
+    show ?thesis
+      using base full by simp
+  next
+    case False
+    have base_none: "base_lay p = None"
+      using compile_procs_layout_domain_exact[OF wf layout] False
+      unfolding layout_domain_exact_def
+      by (cases "base_lay p") auto
+    have full_none: "full_lay p = None"
+      by (rule compile_procs_bodies_outside[OF bodies False]) simp
+    show ?thesis
+      using base_none full_none by simp
+  qed
+qed
+
+
+lemma compile_procs_list_decompose:
+  assumes result:
+    "compile_procs_list Pi ps (\<lambda>_. None) 0 =
+      (nout, full_lay, E, C)"
+  shows "\<exists>nbase base_lay.
+    compile_procs_layout Pi ps (\<lambda>_. None) 0 =
+      (nbase, base_lay) \<and>
+    compile_procs_bodies Pi ps base_lay (\<lambda>_. None) 0 =
+      (nout, full_lay, E, C)"
+proof -
+  obtain nbase base_lay where layout:
+      "compile_procs_layout Pi ps (\<lambda>_. None) 0 =
+        (nbase, base_lay)"
+    by (cases "compile_procs_layout Pi ps (\<lambda>_. None) 0") auto
+  obtain nbody body_lay Ebody Cbody where bodies:
+      "compile_procs_bodies Pi ps base_lay (\<lambda>_. None) 0 =
+        (nbody, body_lay, Ebody, Cbody)"
+    by (cases "compile_procs_bodies Pi ps base_lay
+      (\<lambda>_. None) 0") auto
+  show ?thesis
+    using result layout bodies
+    unfolding compile_procs_list_def
+    by simp
+qed
+
+
 lemma compile_procs_bodies_fragment:
   assumes bodies:
     "compile_procs_bodies \<Pi> ps base_lay in_lay n =
@@ -497,10 +756,383 @@ lemma compile_call_defined:
       {(n, EA_Enter, en)}, {(n, ex, n + 1)})"
 using layout by simp
 
+subsection \<open>Residual commands inside compiled fragments\<close>
+
+type_synonym frame_site = "pp \<times> pp"
+
+inductive control_at ::
+  "proc_table \<Rightarrow> proc_layout \<Rightarrow> IMP2_Proc.com \<Rightarrow> nat \<Rightarrow>
+   IMP2_Proc.com \<Rightarrow> pp \<Rightarrow> frame_site list \<Rightarrow> bool"
+  for Pi :: proc_table and lay :: proc_layout
+where
+  Skip:
+    "control_at Pi lay IMP2_Proc.com.SKIP n
+       IMP2_Proc.com.SKIP n []"
+| Assign:
+    "control_at Pi lay (IMP2_Proc.com.Assign x a) n
+       (IMP2_Proc.com.Assign x a) n []"
+| AssignDone:
+    "control_at Pi lay (IMP2_Proc.com.Assign x a) n
+       IMP2_Proc.com.SKIP (n + 1) []"
+| SeqLeft:
+    "compile Pi lay c1 n = (n1, en1, ex1, E1, C1) \<Longrightarrow>
+     source_com c2 \<Longrightarrow>
+     control_at Pi lay c1 n residual v sites \<Longrightarrow>
+     control_at Pi lay (IMP2_Proc.com.Seq c1 c2) n
+       (IMP2_Proc.com.Seq residual c2) v sites"
+| SeqRight:
+    "compile Pi lay c1 n = (n1, en1, ex1, E1, C1) \<Longrightarrow>
+     control_at Pi lay c2 n1 residual v sites \<Longrightarrow>
+     control_at Pi lay (IMP2_Proc.com.Seq c1 c2) n
+       residual v sites"
+| IfHead:
+    "source_com c1 \<Longrightarrow>
+     source_com c2 \<Longrightarrow>
+     control_at Pi lay (IMP2_Proc.com.If b c1 c2) n
+       (IMP2_Proc.com.If b c1 c2) n []"
+| IfLeft:
+    "control_at Pi lay c1 (n + 1) residual v sites \<Longrightarrow>
+     control_at Pi lay (IMP2_Proc.com.If b c1 c2) n
+       residual v sites"
+| IfRight:
+    "compile Pi lay c1 (n + 1) = (n1, en1, ex1, E1, C1) \<Longrightarrow>
+     control_at Pi lay c2 n1 residual v sites \<Longrightarrow>
+     control_at Pi lay (IMP2_Proc.com.If b c1 c2) n
+       residual v sites"
+| IfDone:
+    "compile Pi lay (IMP2_Proc.com.If b c1 c2) n =
+       (n1, en, ex, E, C) \<Longrightarrow>
+     control_at Pi lay (IMP2_Proc.com.If b c1 c2) n
+       IMP2_Proc.com.SKIP ex []"
+| WhileHead:
+    "source_com body \<Longrightarrow>
+     control_at Pi lay (IMP2_Proc.com.While b body) n
+       (IMP2_Proc.com.While b body) n []"
+| WhileUnfolded:
+    "source_com body \<Longrightarrow>
+     control_at Pi lay (IMP2_Proc.com.While b body) n
+       (IMP2_Proc.com.If b
+         (IMP2_Proc.com.Seq body (IMP2_Proc.com.While b body))
+         IMP2_Proc.com.SKIP) n []"
+| WhileBody:
+    "source_com body \<Longrightarrow>
+     control_at Pi lay body (n + 1) residual v sites \<Longrightarrow>
+     control_at Pi lay (IMP2_Proc.com.While b body) n
+       (IMP2_Proc.com.Seq residual (IMP2_Proc.com.While b body))
+       v sites"
+| WhileDone:
+    "compile Pi lay (IMP2_Proc.com.While b body) n =
+       (n1, en, ex, E, C) \<Longrightarrow>
+     control_at Pi lay (IMP2_Proc.com.While b body) n
+       IMP2_Proc.com.SKIP ex []"
+| ScopeHead:
+    "source_com body \<Longrightarrow>
+     control_at Pi lay (IMP2_Proc.com.Scope body) n
+       (IMP2_Proc.com.Scope body) n []"
+| ScopeBody:
+    "compile Pi lay (IMP2_Proc.com.Scope body) n =
+       (n1, en, scope_ex, E, C) \<Longrightarrow>
+     control_at Pi lay body (n + 1) residual v sites \<Longrightarrow>
+     control_at Pi lay (IMP2_Proc.com.Scope body) n
+       (IMP2_Proc.com.Seq residual IMP2_Proc.com.Restore)
+       v (sites @ [(n, scope_ex)])"
+| ScopeRestore:
+    "compile Pi lay body (n + 1) = (n1, en, body_ex, E, C) \<Longrightarrow>
+     control_at Pi lay (IMP2_Proc.com.Scope body) n
+       IMP2_Proc.com.Restore body_ex [(n, n1)]"
+| ScopeDone:
+    "compile Pi lay (IMP2_Proc.com.Scope body) n =
+       (n1, en, scope_ex, E, C) \<Longrightarrow>
+     control_at Pi lay (IMP2_Proc.com.Scope body) n
+       IMP2_Proc.com.SKIP scope_ex []"
+| CallHead:
+    "control_at Pi lay (IMP2_Proc.com.Call p) n
+       (IMP2_Proc.com.Call p) n []"
+| CallBody:
+    "Pi p = Some body \<Longrightarrow>
+     lay p = Some (proc_en, proc_ex, Ns, Ep, Cp) \<Longrightarrow>
+     compile Pi lay body proc_en =
+       (n1, body_en, proc_ex, E, C) \<Longrightarrow>
+     control_at Pi lay body proc_en residual v sites \<Longrightarrow>
+     control_at Pi lay (IMP2_Proc.com.Call p) n
+       (IMP2_Proc.com.Seq residual IMP2_Proc.com.Restore)
+       v (sites @ [(n, n + 1)])"
+| CallRestore:
+    "lay p = Some (proc_en, proc_ex, Ns, Ep, Cp) \<Longrightarrow>
+     control_at Pi lay (IMP2_Proc.com.Call p) n
+       IMP2_Proc.com.Restore proc_ex [(n, n + 1)]"
+| CallDone:
+    "lay p = Some (proc_en, proc_ex, Ns, Ep, Cp) \<Longrightarrow>
+     control_at Pi lay (IMP2_Proc.com.Call p) n
+       IMP2_Proc.com.SKIP (n + 1) []"
+
+lemma control_at_initial:
+  assumes source: "source_com cmd"
+  shows "control_at Pi lay cmd n cmd n []"
+  using source
+proof (induction cmd arbitrary: n)
+  case SKIP
+  show ?case by (rule control_at.Skip)
+next
+  case Assign
+  show ?case by (rule control_at.Assign)
+next
+  case (Seq c1 c2)
+  obtain n1 en1 ex1 E1 C1 where first:
+      "compile Pi lay c1 n = (n1, en1, ex1, E1, C1)"
+    by (cases "compile Pi lay c1 n") auto
+  have left: "control_at Pi lay c1 n c1 n []"
+    by (rule Seq.IH(1)) (use Seq.prems in simp)
+  show ?case
+    by (rule control_at.SeqLeft[OF first _ left])
+       (use Seq.prems in simp)
+next
+  case If
+  show ?case
+    by (rule control_at.IfHead) (use If.prems in simp_all)
+next
+  case While
+  show ?case
+    by (rule control_at.WhileHead) (use While.prems in simp)
+next
+  case Scope
+  show ?case
+    by (rule control_at.ScopeHead) (use Scope.prems in simp)
+next
+  case Call
+  show ?case by (rule control_at.CallHead)
+next
+  case Restore
+  then show ?case by simp
+qed
+
+lemma compile_endpoint_shape_entry:
+  "(case compile_endpoint_shape lay cmd n of
+      (n', en, ex) \<Rightarrow> en) = n"
+proof (induction cmd arbitrary: n)
+  case SKIP
+  then show ?case by simp
+next
+  case Assign
+  then show ?case by simp
+next
+  case (Seq c1 c2)
+  obtain n1 en1 ex1 where first:
+      "compile_endpoint_shape lay c1 n = (n1, en1, ex1)"
+    by (cases "compile_endpoint_shape lay c1 n") auto
+  obtain n2 en2 ex2 where second:
+      "compile_endpoint_shape lay c2 n1 = (n2, en2, ex2)"
+    by (cases "compile_endpoint_shape lay c2 n1") auto
+  have "en1 = n"
+    using Seq.IH(1)[of n] first by simp
+  then show ?case
+    using first second by simp
+next
+  case If
+  then show ?case by (simp split: prod.splits)
+next
+  case While
+  then show ?case by (simp split: prod.splits)
+next
+  case Scope
+  then show ?case by (simp split: prod.splits)
+next
+  case Call
+  then show ?case by (simp split: option.splits)
+next
+  case Restore
+  then show ?case by simp
+qed
+
+lemma compile_entry_eq:
+  assumes comp: "compile Pi lay cmd n = (n', en, ex, E, C)"
+  shows "en = n"
+proof -
+  have shape:
+      "compile_endpoints Pi lay cmd n =
+        compile_endpoint_shape lay cmd n"
+    by (rule compile_endpoints_eq_shape)
+  show ?thesis
+    using shape compile_endpoint_shape_entry[of lay cmd n] comp
+    unfolding compile_endpoints_def
+    by (cases "compile_endpoint_shape lay cmd n") simp
+qed
+
+lemma compile_procs_list_body:
+  assumes wf: "wf_compile_input Pi ps main"
+      and procs:
+        "compile_procs_list Pi ps (\<lambda>_. None) 0 =
+          (nout, full_lay, Eall, C_all)"
+      and body: "Pi p = Some cmd"
+      and lookup:
+        "full_lay p = Some (en, ex, Ns, Ep, Cp)"
+  shows "\<exists>finish.
+    compile Pi full_lay cmd en = (finish, en, ex, Ep, Cp)"
+proof -
+  obtain nbase base_lay where layout:
+      "compile_procs_layout Pi ps (\<lambda>_. None) 0 =
+        (nbase, base_lay)"
+      and bodies:
+      "compile_procs_bodies Pi ps base_lay (\<lambda>_. None) 0 =
+        (nout, full_lay, Eall, C_all)"
+    using compile_procs_list_decompose[OF procs] by blast
+  have member: "p \<in> set ps"
+    using wf body by (auto simp: wf_compile_input_def)
+  have distinct: "distinct ps"
+    using wf by (auto simp: wf_compile_input_def)
+  have compiled_info:
+      "\<exists>start finish. compile Pi base_lay cmd start =
+        (finish, en, ex, Ep, Cp)"
+    by (rule compile_procs_bodies_lookup[
+          OF distinct _ bodies member body lookup])
+       simp
+  then obtain start finish where compiled_base:
+      "compile Pi base_lay cmd start =
+        (finish, en, ex, Ep, Cp)"
+    by blast
+  have agree: "layouts_agree base_lay full_lay"
+    by (rule compile_procs_pass_layouts_agree[
+          OF wf layout bodies])
+  have same:
+      "compile Pi base_lay cmd start =
+       compile Pi full_lay cmd start"
+    by (rule compile_layouts_agree[OF agree])
+  have start: "start = en"
+    by (rule sym, rule compile_entry_eq[OF compiled_base])
+  have compiled_full:
+      "compile Pi full_lay cmd start =
+        (finish, en, ex, Ep, Cp)"
+    using compiled_base same by simp
+  show ?thesis
+    using compiled_full start by simp
+qed
+
+lemma compile_procs_list_complete:
+  assumes wf: "wf_compile_input Pi ps main"
+      and procs:
+        "compile_procs_list Pi ps (\<lambda>_. None) 0 =
+          (nout, full_lay, Eall, C_all)"
+      and body: "Pi p = Some cmd"
+  shows "\<exists>en ex Ns Ep Cp.
+    full_lay p = Some (en, ex, Ns, Ep, Cp)"
+proof -
+  obtain nbase base_lay where layout:
+      "compile_procs_layout Pi ps (\<lambda>_. None) 0 =
+        (nbase, base_lay)"
+      and bodies:
+      "compile_procs_bodies Pi ps base_lay (\<lambda>_. None) 0 =
+        (nout, full_lay, Eall, C_all)"
+    using compile_procs_list_decompose[OF procs] by blast
+  have member: "p \<in> set ps"
+    using wf body by (auto simp: wf_compile_input_def)
+  have distinct: "distinct ps"
+    using wf by (auto simp: wf_compile_input_def)
+  have defined: "\<forall>q \<in> set ps. Pi q \<noteq> None"
+    using wf by (auto simp: wf_compile_input_def)
+  obtain en ex Ns where base:
+      "base_lay p = Some (en, ex, Ns, {}, {})"
+    using compile_procs_layout_member[
+      OF distinct _ defined layout member]
+    by auto
+  obtain Ns' Ep Cp where full:
+      "full_lay p = Some (en, ex, Ns', Ep, Cp)"
+    using compile_procs_pass_endpoint_agreement[
+      OF wf layout bodies member body base]
+    by blast
+  show ?thesis using full by blast
+qed
+
 subsection \<open>Located CFG execution\<close>
 
 type_synonym cframe = "pp \<times> pp \<times> store"
 type_synonym cconf = "pp \<times> store \<times> cframe list"
+
+fun frames_match ::
+  "frame_site list \<Rightarrow> frame list \<Rightarrow> cframe list \<Rightarrow> bool"
+where
+  "frames_match [] [] [] = True"
+| "frames_match ((call, ret) # sites) (saved # frs)
+     ((call', ret', saved') # stk) =
+     (call = call' \<and> ret = ret' \<and> saved = saved' \<and>
+      frames_match sites frs stk)"
+| "frames_match _ _ _ = False"
+
+definition concrete_program_match ::
+  "proc_table \<Rightarrow> pname list \<Rightarrow> IMP2_Proc.com \<Rightarrow>
+   (IMP2_Proc.com \<times> store \<times> frame list) \<Rightarrow> cconf \<Rightarrow> bool"
+where
+  "concrete_program_match Pi ps main src cf \<longleftrightarrow>
+    (case src of (residual, s, frs) \<Rightarrow>
+     case cf of (v, t, stk) \<Rightarrow>
+       s = t \<and>
+       (\<exists>nproc lay Eproc Cproc nend main_en main_ex Emain Cmain sites.
+          compile_procs_list Pi ps (\<lambda>_. None) 0 =
+            (nproc, lay, Eproc, Cproc) \<and>
+          compile Pi lay main nproc =
+            (nend, main_en, main_ex, Emain, Cmain) \<and>
+          control_at Pi lay main nproc residual v sites \<and>
+          frames_match sites frs stk))"
+
+lemma concrete_program_initial_match:
+  assumes source: "source_com main"
+  shows "concrete_program_match Pi ps main
+    (main, s, []) (cfg_entry (compile_prog Pi ps main), s, [])"
+proof -
+  obtain nproc lay Eproc Cproc where procs:
+      "compile_procs_list Pi ps (\<lambda>_. None) 0 =
+        (nproc, lay, Eproc, Cproc)"
+    by (cases "compile_procs_list Pi ps (\<lambda>_. None) 0") auto
+  obtain nend main_en main_ex Emain Cmain where main_comp:
+      "compile Pi lay main nproc =
+        (nend, main_en, main_ex, Emain, Cmain)"
+    by (cases "compile Pi lay main nproc") auto
+  have entry: "main_en = nproc"
+    by (rule compile_entry_eq[OF main_comp])
+  have control: "control_at Pi lay main nproc main nproc []"
+    by (rule control_at_initial[OF source])
+  show ?thesis
+    unfolding concrete_program_match_def compile_prog_def
+      compile_prog_with_regions_def
+    using procs main_comp entry
+    apply simp
+    apply (rule exI[where x = "[]"])
+    using control
+    apply simp
+    done
+qed
+
+lemma compile_procs_list_fragment:
+  assumes procs:
+    "compile_procs_list Pi ps (\<lambda>_. None) 0 =
+      (nout, full_lay, Eall, C_all)"
+      and lookup:
+    "full_lay p = Some (en, ex, Ns, Ep, Cp)"
+  shows "Ep \<subseteq> Eall \<and> Cp \<subseteq> C_all"
+proof -
+  obtain nbase base_lay where layout:
+      "compile_procs_layout Pi ps (\<lambda>_. None) 0 =
+        (nbase, base_lay)"
+      and bodies:
+      "compile_procs_bodies Pi ps base_lay (\<lambda>_. None) 0 =
+        (nout, full_lay, Eall, C_all)"
+    using compile_procs_list_decompose[OF procs] by blast
+  show ?thesis
+    using compile_procs_bodies_fragment[OF bodies lookup]
+    by auto
+qed
+
+lemma compile_prog_sets:
+  assumes procs:
+    "compile_procs_list Pi ps (\<lambda>_. None) 0 =
+      (nproc, lay, Eproc, Cproc)"
+      and main_comp:
+    "compile Pi lay main nproc =
+      (nend, main_en, main_ex, Emain, Cmain)"
+  shows "edges (compile_prog Pi ps main) = Eproc \<union> Emain"
+    and "combines (compile_prog Pi ps main) = Cproc \<union> Cmain"
+  using procs main_comp
+  unfolding compile_prog_def compile_prog_with_regions_def
+  by simp_all
 
 inductive cstep :: "cfg \<Rightarrow> cconf \<Rightarrow> cconf \<Rightarrow> bool" for g where
   Intra:
@@ -517,6 +1149,1104 @@ inductive cstep :: "cfg \<Rightarrow> cconf \<Rightarrow> cconf \<Rightarrow> bo
     "(call, ex, ret) \<in> combines g \<Longrightarrow>
      cstep g (ex, t, (call, ret, s) # stk)
        (ret, IMP2_Globals.combine_states s t, stk)"
+
+
+lemma cstep_star_single:
+  assumes step: "cstep g cf cf'"
+  shows "star (cstep g) cf cf'"
+  apply (rule star.step)
+   apply (rule step)
+  apply (rule star.refl)
+  done
+
+lemma cstep_nop:
+  assumes edge: "(u, EA_Nop, v) \<in> edges g"
+  shows "cstep g (u, s, stk) (v, s, stk)"
+  by (rule cstep.Intra[OF edge]) simp_all
+
+lemma cstep_assign:
+  assumes edge: "(u, EA_Assign x a, v) \<in> edges g"
+  shows "cstep g (u, s, stk)
+    (v, s(x := IMP2_Expr.aval a s), stk)"
+  by (rule cstep.Intra[OF edge]) simp_all
+
+lemma cstep_assume:
+  assumes edge: "(u, EA_Assume b, v) \<in> edges g"
+      and guard: "IMP2_Expr.bval b s"
+  shows "cstep g (u, s, stk) (v, s, stk)"
+  by (rule cstep.Intra[OF edge]) (simp_all add: guard)
+
+lemma cstep_assume_not:
+  assumes edge: "(u, EA_AssumeNot b, v) \<in> edges g"
+      and guard: "\<not> IMP2_Expr.bval b s"
+  shows "cstep g (u, s, stk) (v, s, stk)"
+  by (rule cstep.Intra[OF edge]) (simp_all add: guard)
+
+lemma cstep_star_nop_right:
+  assumes run: "star (cstep g) cf (u, s, stk)"
+      and edge: "(u, EA_Nop, v) \<in> edges g"
+  shows "star (cstep g) cf (v, s, stk)"
+  by (rule star_trans[OF run cstep_star_single[OF cstep_nop[OF edge]]])
+
+theorem control_finish_simulation:
+  assumes compiled:
+        "compile Pi lay original n = (n', en, ex, E, C)"
+      and edges: "E \<subseteq> edges g"
+      and control:
+        "control_at Pi lay original n residual v sites"
+      and finished: "residual = IMP2_Proc.com.SKIP"
+      and frames: "frames_match (sites @ suffix) frs stk"
+  shows "\<exists>stk'.
+    star (cstep g) (v, s, stk) (ex, s, stk') \<and>
+    frames_match suffix frs stk'"
+  using control finished compiled edges frames
+  by (induction arbitrary: n' en ex E C suffix frs stk
+      rule: control_at.induct;
+      fastforce intro: star.refl cstep_star_single cstep_nop cstep_star_nop_right star_trans
+        split: prod.splits if_splits)
+
+definition proc_layout_sound ::
+  "proc_table \<Rightarrow> proc_layout \<Rightarrow> cfg \<Rightarrow> bool"
+where
+  "proc_layout_sound Pi lay g \<longleftrightarrow>
+    source_pi Pi \<and>
+    (\<forall>p body. Pi p = Some body \<longrightarrow>
+      (\<exists>en ex Ns Ep Cp.
+        lay p = Some (en, ex, Ns, Ep, Cp))) \<and>
+    (\<forall>p body en ex Ns Ep Cp.
+      Pi p = Some body \<longrightarrow>
+      lay p = Some (en, ex, Ns, Ep, Cp) \<longrightarrow>
+      (\<exists>finish.
+        compile Pi lay body en = (finish, en, ex, Ep, Cp)) \<and>
+      Ep \<subseteq> edges g \<and> Cp \<subseteq> combines g)"
+
+theorem control_step_simulation:
+  assumes compiled:
+        "compile Pi lay original n = (n', en, ex, E, C)"
+      and edges: "E \<subseteq> edges g"
+      and combines: "C \<subseteq> combines g"
+      and procedures: "proc_layout_sound Pi lay g"
+      and control:
+        "control_at Pi lay original n residual v sites"
+      and frames: "frames_match (sites @ suffix) frs stk"
+      and step:
+        "pstep Pi (residual, s, frs) (residual', s', frs')"
+  shows "\<exists>v' sites' stk'.
+    star (cstep g) (v, s, stk) (v', s', stk') \<and>
+    control_at Pi lay original n residual' v' sites' \<and>
+    frames_match (sites' @ suffix) frs' stk'"  using control compiled edges combines procedures frames step
+proof (induction arbitrary: n' en ex E C suffix frs stk
+    residual' s' frs' rule: control_at.induct)
+  case Skip
+  then show ?case by (elim SkipSE)
+next
+  case (Assign x a n)
+  have source_result:
+      "(residual', s', frs') =
+       (IMP2_Proc.com.SKIP, s(x := IMP2_Expr.aval a s), frs)"
+    using Assign.prems(6)
+    by (rule AssignSE) simp
+  have shape:
+      "n = en \<and> ex = n + 1 \<and>
+       E = {(n, EA_Assign x a, n + 1)}"
+    using Assign.prems(1) by auto
+  have edge: "(n, EA_Assign x a, n + 1) \<in> edges g"
+    using Assign.prems(2) shape by blast
+  have concrete:
+      "cstep g (n, s, stk)
+        (n + 1, s(x := IMP2_Expr.aval a s), stk)"
+    by (rule cstep_assign[OF edge])
+  have run:
+      "star (cstep g) (n, s, stk)
+        (n + 1, s(x := IMP2_Expr.aval a s), stk)"
+    by (rule cstep_star_single[OF concrete])
+  have located:
+      "control_at Pi lay (IMP2_Proc.com.Assign x a) n
+        IMP2_Proc.com.SKIP (n + 1) []"
+    by (rule control_at.AssignDone)
+  have matched: "frames_match ([] @ suffix) frs stk"
+    using Assign.prems(5) by simp
+  show ?case
+    using source_result run located matched by blast
+next
+  case AssignDone
+  then show ?case by (elim SkipSE)
+next
+  case (SeqLeft c1 n n1 en1 ex1 E1 C1 c2 residual v sites)
+  show ?case
+  proof (rule SeqSE[OF SeqLeft.prems(6)])
+    assume residual_skip: "residual = IMP2_Proc.com.SKIP"
+       and source_result:
+         "(residual', s', frs') = (c2, s, frs)"
+    obtain n2 en2 ex2 E2 C2 where second:
+        "compile Pi lay c2 n1 = (n2, en2, ex2, E2, C2)"
+      by (cases "compile Pi lay c2 n1") auto
+    have parent_edges:
+        "E = E1 \<union>
+          (if ex1 = en2 then {} else {(ex1, EA_Nop, en2)})
+          \<union> E2"
+      using SeqLeft.prems(1) SeqLeft.hyps(1) second by simp
+    have sub_edges: "E1 \<subseteq> edges g"
+      using SeqLeft.prems(2) parent_edges by blast
+    obtain stk1 where body_run:
+        "star (cstep g) (v, s, stk) (ex1, s, stk1)"
+        and body_frames: "frames_match suffix frs stk1"
+      using control_finish_simulation[
+          OF SeqLeft.hyps(1) sub_edges SeqLeft.hyps(3)
+             residual_skip SeqLeft.prems(5)]
+      by blast
+    have entry: "en2 = n1"
+      by (rule compile_entry_eq[OF second])
+    have bridge:
+        "star (cstep g) (ex1, s, stk1) (en2, s, stk1)"
+    proof (cases "ex1 = en2")
+      case True
+      show ?thesis
+        using True star.refl[of "cstep g" "(ex1, s, stk1)"] by simp
+    next
+      case False
+      have edge: "(ex1, EA_Nop, en2) \<in> edges g"
+        using SeqLeft.prems(2) parent_edges False by auto
+      show ?thesis
+        by (rule cstep_star_single, rule cstep_nop[OF edge])
+    qed
+    have run: "star (cstep g) (v, s, stk) (en2, s, stk1)"
+      by (rule star_trans[OF body_run bridge])
+    have next_control:
+        "control_at Pi lay (IMP2_Proc.com.Seq c1 c2) n c2 n1 []"
+      by (rule control_at.SeqRight[OF SeqLeft.hyps(1)])
+         (rule control_at_initial[OF SeqLeft.hyps(2)])
+    show ?case
+      apply (rule exI[of _ en2])
+      apply (rule exI[of _ "[]"])
+      apply (rule exI[of _ stk1])
+      using source_result entry run next_control body_frames
+      apply simp
+      done
+  next
+    fix inner' t frs1
+    assume source_result:
+        "(residual', s', frs') =
+         (IMP2_Proc.com.Seq inner' c2, t, frs1)"
+       and inner_step:
+         "pstep Pi (residual, s, frs) (inner', t, frs1)"
+    obtain n2 en2 ex2 E2 C2 where second:
+        "compile Pi lay c2 n1 = (n2, en2, ex2, E2, C2)"
+      by (cases "compile Pi lay c2 n1") auto
+    have parent_sets:
+        "E = E1 \<union>
+          (if ex1 = en2 then {} else {(ex1, EA_Nop, en2)})
+          \<union> E2 \<and>
+         C = C1 \<union> C2"
+      using SeqLeft.prems(1) SeqLeft.hyps(1) second by simp
+    have sub_edges: "E1 \<subseteq> edges g"
+      using SeqLeft.prems(2) parent_sets by blast
+    have sub_combines: "C1 \<subseteq> combines g"
+      using SeqLeft.prems(3) parent_sets by blast
+    obtain v' sites' stk' where run:
+        "star (cstep g) (v, s, stk) (v', t, stk')"
+        and inner_control:
+          "control_at Pi lay c1 n inner' v' sites'"
+        and matched:
+          "frames_match (sites' @ suffix) frs1 stk'"
+      using SeqLeft.IH[
+          OF SeqLeft.hyps(1) sub_edges sub_combines
+             SeqLeft.prems(4) SeqLeft.prems(5) inner_step]
+      by blast
+    have next_control:
+        "control_at Pi lay (IMP2_Proc.com.Seq c1 c2) n
+          (IMP2_Proc.com.Seq inner' c2) v' sites'"
+      by (rule control_at.SeqLeft[
+            OF SeqLeft.hyps(1) SeqLeft.hyps(2) inner_control])
+    show ?case
+      using source_result run next_control matched by blast
+  qed
+next
+  case (SeqRight c1 n n1 en1 ex1 E1 C1 c2 residual v sites)
+  obtain n2 en2 ex2 E2 C2 where second:
+      "compile Pi lay c2 n1 = (n2, en2, ex2, E2, C2)"
+    by (cases "compile Pi lay c2 n1") auto
+  have parent_sets:
+      "E = E1 \<union>
+        (if ex1 = en2 then {} else {(ex1, EA_Nop, en2)})
+        \<union> E2 \<and>
+       C = C1 \<union> C2"
+    using SeqRight.prems(1) SeqRight.hyps(1) second by simp
+  have sub_edges: "E2 \<subseteq> edges g"
+    using SeqRight.prems(2) parent_sets by blast
+  have sub_combines: "C2 \<subseteq> combines g"
+    using SeqRight.prems(3) parent_sets by blast
+  obtain v' sites' stk' where run:
+      "star (cstep g) (v, s, stk) (v', s', stk')"
+      and inner_control:
+        "control_at Pi lay c2 n1 residual' v' sites'"
+      and matched:
+        "frames_match (sites' @ suffix) frs' stk'"
+    using SeqRight.IH[
+        OF second sub_edges sub_combines SeqRight.prems(4)
+           SeqRight.prems(5) SeqRight.prems(6)]
+    by blast
+  have next_control:
+      "control_at Pi lay (IMP2_Proc.com.Seq c1 c2) n
+        residual' v' sites'"
+    by (rule control_at.SeqRight[
+          OF SeqRight.hyps(1) inner_control])
+  show ?case
+    using run next_control matched by blast
+next
+
+  case (IfHead c1 c2 b n)
+  obtain n1 en1 ex1 E1 C1 where first:
+      "compile Pi lay c1 (n + 1) = (n1, en1, ex1, E1, C1)"
+    by (cases "compile Pi lay c1 (n + 1)") auto
+  obtain n2 en2 ex2 E2 C2 where second:
+      "compile Pi lay c2 n1 = (n2, en2, ex2, E2, C2)"
+    by (cases "compile Pi lay c2 n1") auto
+  have parent_edges:
+      "E = insert (ex1, EA_Nop, n2)
+            (insert (ex2, EA_Nop, n2)
+              (insert (n, EA_Assume b, en1)
+                (insert (n, EA_AssumeNot b, en2) (E1 \<union> E2))))"
+    using IfHead.prems(1) first second by auto
+  show ?case
+  proof (rule IfSE[OF IfHead.prems(6)])
+    assume guard: "IMP2_Expr.bval b s"
+       and source_result: "(residual', s', frs') = (c1, s, frs)"
+    have edge: "(n, EA_Assume b, en1) \<in> edges g"
+      using IfHead.prems(2) parent_edges by blast
+    have run: "star (cstep g) (n, s, stk) (en1, s, stk)"
+      by (rule cstep_star_single, rule cstep_assume[OF edge guard])
+    have entry: "en1 = n + 1"
+      by (rule compile_entry_eq[OF first])
+    have branch:
+        "control_at Pi lay (IMP2_Proc.com.If b c1 c2) n c1 en1 []"
+      apply (rule control_at.IfLeft)
+      using control_at_initial[OF IfHead.hyps(1), of Pi lay "n + 1"] entry
+      apply simp
+      done
+    show ?case
+      apply (rule exI[of _ en1])
+      apply (rule exI[of _ "[]"])
+      apply (rule exI[of _ stk])
+      using source_result run branch IfHead.prems(5)
+      apply simp
+      done
+  next
+    assume guard: "\<not> IMP2_Expr.bval b s"
+       and source_result: "(residual', s', frs') = (c2, s, frs)"
+    have edge: "(n, EA_AssumeNot b, en2) \<in> edges g"
+      using IfHead.prems(2) parent_edges by blast
+    have run: "star (cstep g) (n, s, stk) (en2, s, stk)"
+      by (rule cstep_star_single, rule cstep_assume_not[OF edge guard])
+    have entry: "en2 = n1"
+      by (rule compile_entry_eq[OF second])
+    have branch:
+        "control_at Pi lay (IMP2_Proc.com.If b c1 c2) n c2 en2 []"
+      apply (rule control_at.IfRight[OF first])
+      using control_at_initial[OF IfHead.hyps(2), of Pi lay n1] entry
+      apply simp
+      done
+    show ?case
+      apply (rule exI[of _ en2])
+      apply (rule exI[of _ "[]"])
+      apply (rule exI[of _ stk])
+      using source_result run branch IfHead.prems(5)
+      apply simp
+      done
+  qed
+next
+  case (IfLeft c1 n residual v sites b c2)  obtain n1 en1 ex1 E1 C1 where first:
+      "compile Pi lay c1 (n + 1) = (n1, en1, ex1, E1, C1)"
+    by (cases "compile Pi lay c1 (n + 1)") auto
+  obtain n2 en2 ex2 E2 C2 where second:
+      "compile Pi lay c2 n1 = (n2, en2, ex2, E2, C2)"
+    by (cases "compile Pi lay c2 n1") auto
+  have parent_sets:
+      "E = insert (ex1, EA_Nop, n2)
+            (insert (ex2, EA_Nop, n2)
+              (insert (n, EA_Assume b, en1)
+                (insert (n, EA_AssumeNot b, en2) (E1 \<union> E2))))
+       \<and> C = C1 \<union> C2"
+    using IfLeft.prems(1) first second by auto
+  have sub_edges: "E1 \<subseteq> edges g"
+    using IfLeft.prems(2) parent_sets by blast
+  have sub_combines: "C1 \<subseteq> combines g"
+    using IfLeft.prems(3) parent_sets by blast
+  obtain v' sites' stk' where run:
+      "star (cstep g) (v, s, stk) (v', s', stk')"
+      and inner_control:
+        "control_at Pi lay c1 (n + 1) residual' v' sites'"
+      and matched:
+        "frames_match (sites' @ suffix) frs' stk'"
+    using IfLeft.IH[
+        OF first sub_edges sub_combines IfLeft.prems(4)
+           IfLeft.prems(5) IfLeft.prems(6)]
+    by blast
+  have next_control:
+      "control_at Pi lay (IMP2_Proc.com.If b c1 c2) n
+        residual' v' sites'"
+    by (rule control_at.IfLeft[OF inner_control])
+  show ?case
+    using run next_control matched by blast
+next
+  case (IfRight c1 n n1 en1 ex1 E1 C1 c2 residual v sites b)
+  obtain n2 en2 ex2 E2 C2 where second:
+      "compile Pi lay c2 n1 = (n2, en2, ex2, E2, C2)"
+    by (cases "compile Pi lay c2 n1") auto
+  have parent_sets:
+      "E = insert (ex1, EA_Nop, n2)
+            (insert (ex2, EA_Nop, n2)
+              (insert (n, EA_Assume b, en1)
+                (insert (n, EA_AssumeNot b, en2) (E1 \<union> E2))))
+       \<and> C = C1 \<union> C2"
+    using IfRight.prems(1) IfRight.hyps(1) second by auto
+  have sub_edges: "E2 \<subseteq> edges g"
+    using IfRight.prems(2) parent_sets by blast
+  have sub_combines: "C2 \<subseteq> combines g"
+    using IfRight.prems(3) parent_sets by blast
+  obtain v' sites' stk' where run:
+      "star (cstep g) (v, s, stk) (v', s', stk')"
+      and inner_control:
+        "control_at Pi lay c2 n1 residual' v' sites'"
+      and matched:
+        "frames_match (sites' @ suffix) frs' stk'"
+    using IfRight.IH[
+        OF second sub_edges sub_combines IfRight.prems(4)
+           IfRight.prems(5) IfRight.prems(6)]
+    by blast
+  have next_control:
+      "control_at Pi lay (IMP2_Proc.com.If b c1 c2) n
+        residual' v' sites'"
+    by (rule control_at.IfRight[
+          OF IfRight.hyps(1) inner_control])
+  show ?case
+    using run next_control matched by blast
+next
+  case IfDone
+  then show ?case by (elim SkipSE)
+next
+  case (WhileHead body b n)
+  have source_result:
+      "(residual', s', frs') =
+       (IMP2_Proc.com.If b
+         (IMP2_Proc.com.Seq body (IMP2_Proc.com.While b body))
+         IMP2_Proc.com.SKIP, s, frs)"
+    using WhileHead.prems(6)
+    by (rule WhileSE) simp
+  have run: "star (cstep g) (n, s, stk) (n, s, stk)"
+    by (rule star.refl)
+  have located:
+      "control_at Pi lay (IMP2_Proc.com.While b body) n
+        (IMP2_Proc.com.If b
+          (IMP2_Proc.com.Seq body (IMP2_Proc.com.While b body))
+          IMP2_Proc.com.SKIP) n []"
+    by (rule control_at.WhileUnfolded[OF WhileHead.hyps(1)])
+  show ?case
+    apply (rule exI[of _ n])
+    apply (rule exI[of _ "[]"])
+    apply (rule exI[of _ stk])
+    using source_result run located WhileHead.prems(5)
+    apply simp
+    done
+next
+  case (WhileUnfolded body b n)
+  obtain n1 body_en body_ex Eb Cb where body_comp:
+      "compile Pi lay body (n + 1) =
+       (n1, body_en, body_ex, Eb, Cb)"
+    by (cases "compile Pi lay body (n + 1)") auto
+  have parent_edges:
+      "E = insert (body_ex, EA_Nop, n)
+            (insert (n, EA_Assume b, body_en)
+              (insert (n, EA_AssumeNot b, n1) Eb))"
+    using WhileUnfolded.prems(1) body_comp by auto
+  show ?case
+  proof (rule IfSE[OF WhileUnfolded.prems(6)])
+    assume guard: "IMP2_Expr.bval b s"
+       and source_result:
+         "(residual', s', frs') =
+          (IMP2_Proc.com.Seq body (IMP2_Proc.com.While b body),
+           s, frs)"
+    have edge: "(n, EA_Assume b, body_en) \<in> edges g"
+      using WhileUnfolded.prems(2) parent_edges by blast
+    have run:
+        "star (cstep g) (n, s, stk) (body_en, s, stk)"
+      by (rule cstep_star_single, rule cstep_assume[OF edge guard])
+    have entry: "body_en = n + 1"
+      by (rule compile_entry_eq[OF body_comp])
+    have body_control:
+        "control_at Pi lay body (n + 1) body body_en []"
+      using control_at_initial[OF WhileUnfolded.hyps(1), of Pi lay "n + 1"]
+        entry by simp
+    have located:
+        "control_at Pi lay (IMP2_Proc.com.While b body) n
+          (IMP2_Proc.com.Seq body (IMP2_Proc.com.While b body))
+          body_en []"
+      by (rule control_at.WhileBody[
+            OF WhileUnfolded.hyps(1) body_control])
+    show ?case
+      apply (rule exI[of _ body_en])
+      apply (rule exI[of _ "[]"])
+      apply (rule exI[of _ stk])
+      using source_result run located WhileUnfolded.prems(5)
+      apply simp
+      done
+  next
+    assume guard: "\<not> IMP2_Expr.bval b s"
+       and source_result:
+         "(residual', s', frs') = (IMP2_Proc.com.SKIP, s, frs)"
+    have edge: "(n, EA_AssumeNot b, n1) \<in> edges g"
+      using WhileUnfolded.prems(2) parent_edges by blast
+    have run: "star (cstep g) (n, s, stk) (n1, s, stk)"
+      by (rule cstep_star_single, rule cstep_assume_not[OF edge guard])
+    have exit: "ex = n1"
+      using WhileUnfolded.prems(1) body_comp by auto
+    have finished:
+        "control_at Pi lay (IMP2_Proc.com.While b body) n
+          IMP2_Proc.com.SKIP ex []"
+      by (rule control_at.WhileDone[OF WhileUnfolded.prems(1)])
+    have located:
+        "control_at Pi lay (IMP2_Proc.com.While b body) n
+          IMP2_Proc.com.SKIP n1 []"
+      using finished exit by simp
+    show ?case
+      apply (rule exI[of _ n1])
+      apply (rule exI[of _ "[]"])
+      apply (rule exI[of _ stk])
+      using source_result run located WhileUnfolded.prems(5)
+      apply simp
+      done
+  qed
+next
+  case (WhileBody body n residual v sites b)
+  obtain n1 body_en body_ex Eb Cb where body_comp:
+      "compile Pi lay body (n + 1) =
+       (n1, body_en, body_ex, Eb, Cb)"
+    by (cases "compile Pi lay body (n + 1)") auto
+  have parent_sets:
+      "E = insert (body_ex, EA_Nop, n)
+            (insert (n, EA_Assume b, body_en)
+              (insert (n, EA_AssumeNot b, n1) Eb))
+       \<and> C = Cb"
+    using WhileBody.prems(1) body_comp by auto
+  have sub_edges: "Eb \<subseteq> edges g"
+    using WhileBody.prems(2) parent_sets by blast
+  have sub_combines: "Cb \<subseteq> combines g"
+    using WhileBody.prems(3) parent_sets by blast
+  show ?case
+  proof (rule SeqSE[OF WhileBody.prems(6)])
+    assume residual_skip: "residual = IMP2_Proc.com.SKIP"
+       and source_result:
+         "(residual', s', frs') =
+          (IMP2_Proc.com.While b body, s, frs)"
+    obtain stk1 where body_run:
+        "star (cstep g) (v, s, stk) (body_ex, s, stk1)"
+        and body_frames: "frames_match suffix frs stk1"
+      using control_finish_simulation[
+          OF body_comp sub_edges WhileBody.hyps(2)
+             residual_skip WhileBody.prems(5)]
+      by blast
+    have back_edge: "(body_ex, EA_Nop, n) \<in> edges g"
+      using WhileBody.prems(2) parent_sets by blast
+    have back_run:
+        "star (cstep g) (body_ex, s, stk1) (n, s, stk1)"
+      by (rule cstep_star_single, rule cstep_nop[OF back_edge])
+    have run: "star (cstep g) (v, s, stk) (n, s, stk1)"
+      by (rule star_trans[OF body_run back_run])
+    have located:
+        "control_at Pi lay (IMP2_Proc.com.While b body) n
+          (IMP2_Proc.com.While b body) n []"
+      by (rule control_at.WhileHead[OF WhileBody.hyps(1)])
+    show ?case
+      apply (rule exI[of _ n])
+      apply (rule exI[of _ "[]"])
+      apply (rule exI[of _ stk1])
+      using source_result run located body_frames
+      apply simp
+      done
+  next
+    fix inner' t frs1
+    assume source_result:
+        "(residual', s', frs') =
+         (IMP2_Proc.com.Seq inner' (IMP2_Proc.com.While b body),
+          t, frs1)"
+       and inner_step:
+         "pstep Pi (residual, s, frs) (inner', t, frs1)"
+    obtain v' sites' stk' where run:
+        "star (cstep g) (v, s, stk) (v', t, stk')"
+        and inner_control:
+          "control_at Pi lay body (n + 1) inner' v' sites'"
+        and matched:
+          "frames_match (sites' @ suffix) frs1 stk'"
+      using WhileBody.IH[
+          OF body_comp sub_edges sub_combines WhileBody.prems(4)
+             WhileBody.prems(5) inner_step]
+      by blast
+    have located:
+        "control_at Pi lay (IMP2_Proc.com.While b body) n
+          (IMP2_Proc.com.Seq inner' (IMP2_Proc.com.While b body))
+          v' sites'"
+      by (rule control_at.WhileBody[
+            OF WhileBody.hyps(1) inner_control])
+    show ?case
+      using source_result run located matched by blast
+  qed
+next
+  case WhileDone
+  then show ?case by (elim SkipSE)
+next
+  case (ScopeHead body n)
+  have source_result:
+      "(residual', s', frs') =
+       (IMP2_Proc.com.Seq body IMP2_Proc.com.Restore,
+        enter_state s, s # frs)"
+    using ScopeHead.prems(6)
+    by (rule ScopeSE) simp
+  obtain n1 body_en body_ex Eb Cb where body_comp:
+      "compile Pi lay body (n + 1) =
+       (n1, body_en, body_ex, Eb, Cb)"
+    by (cases "compile Pi lay body (n + 1)") auto
+  have shape:
+      "ex = n1 \<and>
+       (n, EA_Enter, body_en) \<in> E \<and>
+       (n, body_ex, n1) \<in> C"
+    using ScopeHead.prems(1) body_comp by auto
+  have enter_edge:
+      "(n, EA_Enter, body_en) \<in> edges g"
+    using ScopeHead.prems(2) shape by blast
+  have combine:
+      "(n, body_ex, n1) \<in> combines g"
+    using ScopeHead.prems(3) shape by blast
+  have concrete:
+      "cstep g (n, s, stk)
+        (body_en, enter_state s, (n, n1, s) # stk)"
+    by (rule cstep.Call[OF enter_edge combine])
+  have run:
+      "star (cstep g) (n, s, stk)
+        (body_en, enter_state s, (n, n1, s) # stk)"
+    by (rule cstep_star_single[OF concrete])
+  have entry: "body_en = n + 1"
+    by (rule compile_entry_eq[OF body_comp])
+  have body_control:
+      "control_at Pi lay body (n + 1) body body_en []"
+    using control_at_initial[OF ScopeHead.hyps(1), of Pi lay "n + 1"]
+      entry by simp
+  have raw_location:
+      "control_at Pi lay (IMP2_Proc.com.Scope body) n
+        (IMP2_Proc.com.Seq body IMP2_Proc.com.Restore)
+        body_en ([] @ [(n, ex)])"
+    by (rule control_at.ScopeBody[
+          OF ScopeHead.prems(1) body_control])
+  have located:
+      "control_at Pi lay (IMP2_Proc.com.Scope body) n
+        (IMP2_Proc.com.Seq body IMP2_Proc.com.Restore)
+        body_en [(n, n1)]"
+    using raw_location shape by simp
+  have matched:
+      "frames_match ([(n, n1)] @ suffix) (s # frs)
+        ((n, n1, s) # stk)"
+    using ScopeHead.prems(5) by simp
+  show ?case
+    apply (rule exI[of _ body_en])
+    apply (rule exI[of _ "[(n, n1)]"])
+    apply (rule exI[of _ "(n, n1, s) # stk"])
+    using source_result run located matched
+    apply simp
+    done
+next
+  case (ScopeBody body n n1 en scope_ex E0 C0 residual v sites)
+  obtain body_n body_en body_ex Eb Cb where body_comp:
+      "compile Pi lay body (n + 1) =
+       (body_n, body_en, body_ex, Eb, Cb)"
+    by (cases "compile Pi lay body (n + 1)") auto
+  have parent_shape:
+      "scope_ex = body_n \<and>
+       E = insert (n, EA_Enter, body_en) Eb \<and>
+       C = insert (n, body_ex, body_n) Cb"
+    using ScopeBody.prems(1) ScopeBody.hyps(1) body_comp by auto
+  have sub_edges: "Eb \<subseteq> edges g"
+    using ScopeBody.prems(2) parent_shape by blast
+  have sub_combines: "Cb \<subseteq> combines g"
+    using ScopeBody.prems(3) parent_shape by blast
+  have frame_assoc:
+      "(sites @ [(n, scope_ex)]) @ suffix =
+       sites @ ([(n, scope_ex)] @ suffix)"
+    by simp
+  show ?case
+  proof (rule SeqSE[OF ScopeBody.prems(6)])
+    assume residual_skip: "residual = IMP2_Proc.com.SKIP"
+       and source_result:
+         "(residual', s', frs') =
+          (IMP2_Proc.com.Restore, s, frs)"
+    have input_frames:
+        "frames_match
+          (sites @ ([(n, scope_ex)] @ suffix)) frs stk"
+      using ScopeBody.prems(5) frame_assoc by simp
+    obtain stk1 where body_run:
+        "star (cstep g) (v, s, stk) (body_ex, s, stk1)"
+        and body_frames:
+          "frames_match ([(n, scope_ex)] @ suffix) frs stk1"
+      using control_finish_simulation[
+          OF body_comp sub_edges ScopeBody.hyps(2)
+             residual_skip input_frames]
+      by blast
+    have raw_location:
+        "control_at Pi lay (IMP2_Proc.com.Scope body) n
+          IMP2_Proc.com.Restore body_ex [(n, body_n)]"
+      by (rule control_at.ScopeRestore[OF body_comp])
+    have located:
+        "control_at Pi lay (IMP2_Proc.com.Scope body) n
+          IMP2_Proc.com.Restore body_ex [(n, scope_ex)]"
+      using raw_location parent_shape by simp
+    show ?case
+      apply (rule exI[of _ body_ex])
+      apply (rule exI[of _ "[(n, scope_ex)]"])
+      apply (rule exI[of _ stk1])
+      using source_result body_run located body_frames
+      apply simp
+      done
+  next
+    fix inner' t frs1
+    assume source_result:
+        "(residual', s', frs') =
+         (IMP2_Proc.com.Seq inner' IMP2_Proc.com.Restore,
+          t, frs1)"
+       and inner_step:
+         "pstep Pi (residual, s, frs) (inner', t, frs1)"
+    have input_frames:
+        "frames_match
+          (sites @ ([(n, scope_ex)] @ suffix)) frs stk"
+      using ScopeBody.prems(5) frame_assoc by simp
+    obtain v' inner_sites stk' where run:
+        "star (cstep g) (v, s, stk) (v', t, stk')"
+        and inner_control:
+          "control_at Pi lay body (n + 1) inner' v' inner_sites"
+        and matched:
+          "frames_match
+            (inner_sites @ ([(n, scope_ex)] @ suffix))
+            frs1 stk'"
+      using ScopeBody.IH[
+          OF body_comp sub_edges sub_combines ScopeBody.prems(4)
+             input_frames inner_step]
+      by blast
+    have raw_location:
+        "control_at Pi lay (IMP2_Proc.com.Scope body) n
+          (IMP2_Proc.com.Seq inner' IMP2_Proc.com.Restore)
+          v' (inner_sites @ [(n, scope_ex)])"
+      by (rule control_at.ScopeBody[
+            OF ScopeBody.hyps(1) inner_control])
+    have output_frames:
+        "frames_match
+          ((inner_sites @ [(n, scope_ex)]) @ suffix)
+          frs1 stk'"
+      using matched by simp
+    show ?case
+      using source_result run raw_location output_frames by blast
+  qed
+next
+  case (ScopeRestore body n body_n body_en body_ex Eb Cb)
+  have parent_shape:
+      "ex = body_n \<and>
+       (n, body_ex, body_n) \<in> C"
+    using ScopeRestore.prems(1) ScopeRestore.hyps(1) by auto
+  have combine: "(n, body_ex, body_n) \<in> combines g"
+    using ScopeRestore.prems(3) parent_shape by blast
+  show ?case
+  proof (rule RestoreSE[OF ScopeRestore.prems(6)])
+    fix saved outer
+    assume source_frames: "frs = saved # outer"
+       and source_result:
+         "(residual', s', frs') =
+          (IMP2_Proc.com.SKIP,
+           IMP2_Globals.combine_states saved s, outer)"
+    have stack_shape:
+        "\<exists>stk0.
+          stk = (n, body_n, saved) # stk0 \<and>
+          frames_match suffix outer stk0"
+      using ScopeRestore.prems(5) source_frames
+      by (cases stk) auto
+    then obtain stk0 where concrete_stack:
+        "stk = (n, body_n, saved) # stk0"
+        and outer_frames: "frames_match suffix outer stk0"
+      by blast
+    have concrete:
+        "cstep g (body_ex, s, stk)
+          (body_n, IMP2_Globals.combine_states saved s, stk0)"
+      unfolding concrete_stack
+      by (rule cstep.Return[OF combine])
+    have run:
+        "star (cstep g) (body_ex, s, stk)
+          (body_n, IMP2_Globals.combine_states saved s, stk0)"
+      by (rule cstep_star_single[OF concrete])
+    have finished:
+        "control_at Pi lay (IMP2_Proc.com.Scope body) n
+          IMP2_Proc.com.SKIP ex []"
+      by (rule control_at.ScopeDone[OF ScopeRestore.prems(1)])
+    have located:
+        "control_at Pi lay (IMP2_Proc.com.Scope body) n
+          IMP2_Proc.com.SKIP body_n []"
+      using finished parent_shape by simp
+    have result_cmd: "residual' = IMP2_Proc.com.SKIP"
+      and result_store:
+        "s' = IMP2_Globals.combine_states saved s"
+      and result_frames: "frs' = outer"
+      using source_result by simp_all
+    show ?case
+      apply (rule exI[of _ body_n])
+      apply (rule exI[of _ "[]"])
+      apply (rule exI[of _ stk0])
+      apply (intro conjI)
+       apply (subst result_store)
+       apply (rule run)
+       using result_cmd located apply simp
+      using result_frames outer_frames apply simp
+      done
+  qed
+next
+  case ScopeDone
+  then show ?case by (elim SkipSE)
+next
+  case (CallHead p n)
+  show ?case
+  proof (rule CallSE[OF CallHead.prems(6)])
+    fix body
+    assume body: "Pi p = Some body"
+       and source_result:
+         "(residual', s', frs') =
+          (IMP2_Proc.com.Seq body IMP2_Proc.com.Restore,
+           enter_state s, s # frs)"
+    have source_pi: "source_pi Pi"
+      using CallHead.prems(4)
+      unfolding proc_layout_sound_def
+      by (elim conjE) assumption
+    have source_body: "source_com body"
+      using source_pi body unfolding source_pi_def by auto
+    have layout_complete:
+        "\<forall>p body. Pi p = Some body \<longrightarrow>
+          (\<exists>en ex Ns Ep Cp.
+            lay p = Some (en, ex, Ns, Ep, Cp))"
+      using CallHead.prems(4)
+      unfolding proc_layout_sound_def
+      by (elim conjE) assumption
+    obtain proc_en proc_ex Ns Ep Cp where lookup:
+        "lay p = Some (proc_en, proc_ex, Ns, Ep, Cp)"
+      using layout_complete[rule_format, OF body] by blast
+    have layout_fragments:
+        "\<forall>p body en ex Ns Ep Cp.
+          Pi p = Some body \<longrightarrow>
+          lay p = Some (en, ex, Ns, Ep, Cp) \<longrightarrow>
+          (\<exists>finish.
+            compile Pi lay body en =
+              (finish, en, ex, Ep, Cp)) \<and>
+          Ep \<subseteq> edges g \<and> Cp \<subseteq> combines g"
+      using CallHead.prems(4)
+      unfolding proc_layout_sound_def
+      by (elim conjE) assumption
+    obtain finish where body_comp:
+        "compile Pi lay body proc_en =
+         (finish, proc_en, proc_ex, Ep, Cp)"
+      using layout_fragments[rule_format, OF body lookup] by blast
+    have call_shape:
+        "(n, EA_Enter, proc_en) \<in> E \<and>
+         (n, proc_ex, n + 1) \<in> C"
+      using CallHead.prems(1) lookup by auto
+    have enter_edge:
+        "(n, EA_Enter, proc_en) \<in> edges g"
+      using CallHead.prems(2) call_shape by blast
+    have combine:
+        "(n, proc_ex, n + 1) \<in> combines g"
+      using CallHead.prems(3) call_shape by blast
+    have concrete:
+        "cstep g (n, s, stk)
+          (proc_en, enter_state s, (n, n + 1, s) # stk)"
+      by (rule cstep.Call[OF enter_edge combine])
+    have run:
+        "star (cstep g) (n, s, stk)
+          (proc_en, enter_state s, (n, n + 1, s) # stk)"
+      by (rule cstep_star_single[OF concrete])
+    have body_control:
+        "control_at Pi lay body proc_en body proc_en []"
+      by (rule control_at_initial[OF source_body])
+    have raw_location:
+        "control_at Pi lay (IMP2_Proc.com.Call p) n
+          (IMP2_Proc.com.Seq body IMP2_Proc.com.Restore)
+          proc_en ([] @ [(n, n + 1)])"
+      by (rule control_at.CallBody[
+            OF body lookup body_comp body_control])
+    have located:
+        "control_at Pi lay (IMP2_Proc.com.Call p) n
+          (IMP2_Proc.com.Seq body IMP2_Proc.com.Restore)
+          proc_en [(n, n + 1)]"
+      using raw_location by simp
+    have matched:
+        "frames_match ([(n, n + 1)] @ suffix) (s # frs)
+          ((n, n + 1, s) # stk)"
+      using CallHead.prems(5) by simp
+    show ?case
+      apply (rule exI[of _ proc_en])
+      apply (rule exI[of _ "[(n, n + 1)]"])
+      apply (rule exI[of _ "(n, n + 1, s) # stk"])
+      using source_result run located matched
+      apply simp
+      done
+  qed
+next
+  case (CallBody p body proc_en proc_ex Ns Ep Cp n1 body_en Eb Cb
+      residual v sites n)
+  have proc_sound:
+      "(\<exists>finish.
+         compile Pi lay body proc_en =
+           (finish, proc_en, proc_ex, Ep, Cp)) \<and>
+       Ep \<subseteq> edges g \<and> Cp \<subseteq> combines g"
+    using CallBody.prems(4) CallBody.hyps(1,2)
+    unfolding proc_layout_sound_def by blast
+  then obtain finish where canonical:
+      "compile Pi lay body proc_en =
+       (finish, proc_en, proc_ex, Ep, Cp)"
+      and proc_edges: "Ep \<subseteq> edges g"
+      and proc_combines: "Cp \<subseteq> combines g"
+    by blast
+  have output_eq: "Eb = Ep \<and> Cb = Cp"
+    using CallBody.hyps(3) canonical by simp
+  have sub_edges: "Eb \<subseteq> edges g"
+    using proc_edges output_eq by simp
+  have sub_combines: "Cb \<subseteq> combines g"
+    using proc_combines output_eq by simp
+  have frame_assoc:
+      "(sites @ [(n, n + 1)]) @ suffix =
+       sites @ ([(n, n + 1)] @ suffix)"
+    by simp
+  show ?case
+  proof (rule SeqSE[OF CallBody.prems(6)])
+    assume residual_skip: "residual = IMP2_Proc.com.SKIP"
+       and source_result:
+         "(residual', s', frs') =
+          (IMP2_Proc.com.Restore, s, frs)"
+    have input_frames:
+        "frames_match
+          (sites @ ([(n, n + 1)] @ suffix)) frs stk"
+      using CallBody.prems(5) frame_assoc by simp
+    obtain stk1 where body_run:
+        "star (cstep g) (v, s, stk) (proc_ex, s, stk1)"
+        and body_frames:
+          "frames_match ([(n, n + 1)] @ suffix) frs stk1"
+      using control_finish_simulation[
+          OF CallBody.hyps(3) sub_edges CallBody.hyps(4)
+             residual_skip input_frames]
+      by blast
+    have located:
+        "control_at Pi lay (IMP2_Proc.com.Call p) n
+          IMP2_Proc.com.Restore proc_ex [(n, n + 1)]"
+      using CallBody.hyps(2)
+      by (rule control_at.CallRestore)
+    show ?case
+      apply (rule exI[of _ proc_ex])
+      apply (rule exI[of _ "[(n, n + 1)]"])
+      apply (rule exI[of _ stk1])
+      using source_result body_run located body_frames
+      apply simp
+      done
+  next
+    fix inner' t frs1
+    assume source_result:
+        "(residual', s', frs') =
+         (IMP2_Proc.com.Seq inner' IMP2_Proc.com.Restore,
+          t, frs1)"
+       and inner_step:
+         "pstep Pi (residual, s, frs) (inner', t, frs1)"
+    have input_frames:
+        "frames_match
+          (sites @ ([(n, n + 1)] @ suffix)) frs stk"
+      using CallBody.prems(5) frame_assoc by simp
+    obtain v' inner_sites stk' where run:
+        "star (cstep g) (v, s, stk) (v', t, stk')"
+        and inner_control:
+          "control_at Pi lay body proc_en inner' v' inner_sites"
+        and matched:
+          "frames_match
+            (inner_sites @ ([(n, n + 1)] @ suffix))
+            frs1 stk'"
+      using CallBody.IH[
+          OF CallBody.hyps(3) sub_edges sub_combines CallBody.prems(4)
+             input_frames inner_step]
+      by blast
+    have raw_location:
+        "control_at Pi lay (IMP2_Proc.com.Call p) n
+          (IMP2_Proc.com.Seq inner' IMP2_Proc.com.Restore)
+          v' (inner_sites @ [(n, n + 1)])"
+      by (rule control_at.CallBody[
+            OF CallBody.hyps(1) CallBody.hyps(2)
+               CallBody.hyps(3) inner_control])
+    have output_frames:
+        "frames_match
+          ((inner_sites @ [(n, n + 1)]) @ suffix)
+          frs1 stk'"
+      using matched by simp
+    show ?case
+      using source_result run raw_location output_frames by blast
+  qed
+next
+  case (CallRestore p proc_en proc_ex Ns Ep Cp n)
+  have call_shape: "(n, proc_ex, n + 1) \<in> C"
+    using CallRestore.prems(1) CallRestore.hyps(1) by auto
+  have combine: "(n, proc_ex, n + 1) \<in> combines g"
+    using CallRestore.prems(3) call_shape by blast
+  show ?case
+  proof (rule RestoreSE[OF CallRestore.prems(6)])
+    fix saved outer
+    assume source_frames: "frs = saved # outer"
+       and source_result:
+         "(residual', s', frs') =
+          (IMP2_Proc.com.SKIP,
+           IMP2_Globals.combine_states saved s, outer)"
+    have stack_shape:
+        "\<exists>stk0.
+          stk = (n, n + 1, saved) # stk0 \<and>
+          frames_match suffix outer stk0"
+      using CallRestore.prems(5) source_frames
+      by (cases stk) auto
+    then obtain stk0 where concrete_stack:
+        "stk = (n, n + 1, saved) # stk0"
+        and outer_frames: "frames_match suffix outer stk0"
+      by blast
+    have concrete:
+        "cstep g (proc_ex, s, stk)
+          (n + 1, IMP2_Globals.combine_states saved s, stk0)"
+      unfolding concrete_stack
+      by (rule cstep.Return[OF combine])
+    have run:
+        "star (cstep g) (proc_ex, s, stk)
+          (n + 1, IMP2_Globals.combine_states saved s, stk0)"
+      by (rule cstep_star_single[OF concrete])
+    have located:
+        "control_at Pi lay (IMP2_Proc.com.Call p) n
+          IMP2_Proc.com.SKIP (n + 1) []"
+      using CallRestore.hyps(1)
+      by (rule control_at.CallDone)
+    have result_cmd: "residual' = IMP2_Proc.com.SKIP"
+      and result_store:
+        "s' = IMP2_Globals.combine_states saved s"
+      and result_frames: "frs' = outer"
+      using source_result by simp_all
+    show ?case
+      apply (rule exI[of _ "n + 1"])
+      apply (rule exI[of _ "[]"])
+      apply (rule exI[of _ stk0])
+      apply (intro conjI)
+       apply (subst result_store)
+       apply (rule run)
+      using result_cmd located apply simp
+      using result_frames outer_frames apply simp
+      done
+  qed
+next
+  case CallDone
+  then show ?case by (elim SkipSE)
+qed
+
+theorem concrete_program_step_match:
+  assumes wf: "wf_compile_input Pi ps main"
+      and matched: "concrete_program_match Pi ps main src cf"
+      and step: "pstep Pi src src'"
+  shows "\<exists>cf'.
+    star (cstep (compile_prog Pi ps main)) cf cf' \<and>
+    concrete_program_match Pi ps main src' cf'"
+proof -
+  obtain residual s frs where src: "src = (residual, s, frs)"
+    by (cases src) auto
+  obtain residual' s' frs' where src':
+      "src' = (residual', s', frs')"
+    by (cases src') auto
+  obtain v t stk where cf: "cf = (v, t, stk)"
+    by (cases cf) auto
+  obtain nproc lay Eproc Cproc nend main_en main_ex Emain Cmain sites
+    where store: "s = t"
+      and procs:
+        "compile_procs_list Pi ps (\<lambda>_. None) 0 =
+          (nproc, lay, Eproc, Cproc)"
+      and main_comp:
+        "compile Pi lay main nproc =
+          (nend, main_en, main_ex, Emain, Cmain)"
+      and control:
+        "control_at Pi lay main nproc residual v sites"
+      and frames: "frames_match sites frs stk"
+    using matched
+    unfolding concrete_program_match_def src cf
+    by auto
+  have edge_sets:
+      "edges (compile_prog Pi ps main) = Eproc \<union> Emain"
+    by (rule compile_prog_sets(1)[OF procs main_comp])
+  have combine_sets:
+      "combines (compile_prog Pi ps main) = Cproc \<union> Cmain"
+    by (rule compile_prog_sets(2)[OF procs main_comp])
+  have main_edges:
+      "Emain \<subseteq> edges (compile_prog Pi ps main)"
+    unfolding edge_sets by blast
+  have main_combines:
+      "Cmain \<subseteq> combines (compile_prog Pi ps main)"
+    unfolding combine_sets by blast
+  have layout_sound:
+      "proc_layout_sound Pi lay (compile_prog Pi ps main)"
+  proof (unfold proc_layout_sound_def, intro conjI)
+    show "source_pi Pi"
+      using wf unfolding wf_compile_input_def by blast
+    show "\<forall>p body. Pi p = Some body \<longrightarrow>
+      (\<exists>en ex Ns Ep Cp.
+        lay p = Some (en, ex, Ns, Ep, Cp))"
+    proof (intro allI impI)
+      fix p body
+      assume body: "Pi p = Some body"
+      show "\<exists>en ex Ns Ep Cp.
+        lay p = Some (en, ex, Ns, Ep, Cp)"
+        using compile_procs_list_complete[OF wf procs body] .
+    qed
+    show "\<forall>p body en ex Ns Ep Cp.
+      Pi p = Some body \<longrightarrow>
+      lay p = Some (en, ex, Ns, Ep, Cp) \<longrightarrow>
+      (\<exists>finish.
+        compile Pi lay body en = (finish, en, ex, Ep, Cp)) \<and>
+      Ep \<subseteq> edges (compile_prog Pi ps main) \<and>
+      Cp \<subseteq> combines (compile_prog Pi ps main)"
+    proof (intro allI impI)
+      fix p body en ex Ns Ep Cp
+      assume body: "Pi p = Some body"
+      assume lookup: "lay p = Some (en, ex, Ns, Ep, Cp)"
+      obtain finish where compiled_body:
+          "compile Pi lay body en = (finish, en, ex, Ep, Cp)"
+        using compile_procs_list_body[OF wf procs body lookup] by blast
+      have fragment: "Ep \<subseteq> Eproc \<and> Cp \<subseteq> Cproc"
+        by (rule compile_procs_list_fragment[OF procs lookup])
+      show "(\<exists>finish.
+          compile Pi lay body en = (finish, en, ex, Ep, Cp)) \<and>
+          Ep \<subseteq> edges (compile_prog Pi ps main) \<and>
+          Cp \<subseteq> combines (compile_prog Pi ps main)"
+        using compiled_body fragment edge_sets combine_sets by blast
+    qed
+  qed
+  have source_step:
+      "pstep Pi (residual, s, frs) (residual', s', frs')"
+    using step unfolding src src' .
+  have frames_suffix: "frames_match (sites @ []) frs stk"
+    using frames by simp
+  obtain v' sites' stk' where run:
+      "star (cstep (compile_prog Pi ps main))
+        (v, s, stk) (v', s', stk')"
+      and control':
+        "control_at Pi lay main nproc residual' v' sites'"
+      and frames': "frames_match sites' frs' stk'"
+    using control_step_simulation[
+      OF main_comp main_edges main_combines layout_sound
+        control frames_suffix source_step]
+    by auto
+  show ?thesis
+  proof (rule exI[where x = "(v', s', stk')"], intro conjI)
+    show "star (cstep (compile_prog Pi ps main)) cf (v', s', stk')"
+      using run store unfolding cf by simp
+    show "concrete_program_match Pi ps main src' (v', s', stk')"
+      unfolding concrete_program_match_def src'
+      using procs main_comp control' frames'
+      by auto
+  qed
+qed
 
 lemma edge_step_mem_edge_collect:
   assumes "edge_step a s = Some t"
@@ -917,5 +2647,99 @@ proof -
 qed
 
 end
+
+theorem concrete_source_reaches_side_analyse_eff:
+  fixes s0 :: "'a::sound_domain abs_state"
+    and etf :: "('g::finite, 'a) effectful_domain_transfer"
+    and gseed :: 'g
+  assumes wf: "wf_compile_input Pi ps main"
+      and run: "psteps Pi (main, s, []) src'"
+      and se: "sound_effectful_transfer etf"
+      and tfm:
+        "threefold_mono
+          (side_cfg_T_eff (compile_prog Pi ps main) etf bot s0 gseed)"
+      and cone: "cone_compatible_etf etf"
+      and init: "s \<in> \<lbrakk>s0\<rbrakk>"
+      and dom:
+        "\<And>v.
+          cfg_reaches (compile_prog Pi ps main)
+            (cfg_entry (compile_prog Pi ps main)) v \<Longrightarrow>
+          side_cfg_solve_dom_eff
+            (compile_prog Pi ps main) etf bot s0 gseed v"
+  shows "\<exists>v t stk.
+    concrete_program_match Pi ps main src' (v, t, stk) \<and>
+    t \<in> \<lbrakk>side_analyse_eff Pi ps main etf bot s0 gseed v\<rbrakk>"
+proof -
+  have source_main: "source_com main"
+    using wf unfolding wf_compile_input_def by blast
+  interpret sim: compiled_source_simulation
+      Pi ps main "compile_prog Pi ps main"
+      "concrete_program_match Pi ps main"
+  proof
+    show "compile_prog Pi ps main = compile_prog Pi ps main"
+      by simp
+    show "wf_compile_input Pi ps main"
+      by (rule wf)
+    fix t
+    show "concrete_program_match Pi ps main
+      (main, t, []) (cfg_entry (compile_prog Pi ps main), t, [])"
+      by (rule concrete_program_initial_match[OF source_main])
+    fix source source' concrete
+    assume matched:
+        "concrete_program_match Pi ps main source concrete"
+       and stepped: "pstep Pi source source'"
+    show "\<exists>concrete'.
+      star (cstep (compile_prog Pi ps main)) concrete concrete' \<and>
+      concrete_program_match Pi ps main source' concrete'"
+      by (rule concrete_program_step_match[OF wf matched stepped])
+  qed
+  show ?thesis
+    by (rule sim.source_reaches_side_analyse_eff[
+          OF run se tfm cone init dom])
+qed
+
+locale source_to_analysis_bridge =
+  fixes Pi :: proc_table
+    and ps :: "pname list"
+    and main :: IMP2_Proc.com
+    and g :: cfg
+    and s :: store
+    and src' :: "(IMP2_Proc.com \<times> store \<times> frame list)"
+    and etf :: "('g::finite, 'a::sound_domain) effectful_domain_transfer"
+    and s0 :: "'a abs_state"
+    and gseed :: 'g
+  assumes g_def: "g = compile_prog Pi ps main"
+      and wf: "wf_compile_input Pi ps main"
+      and run: "psteps Pi (main, s, []) src'"
+      and se: "sound_effectful_transfer etf"
+      and tfm: "threefold_mono (side_cfg_T_eff g etf bot s0 gseed)"
+      and cone: "cone_compatible_etf etf"
+      and init: "s \<in> \<lbrakk>s0\<rbrakk>"
+begin
+
+theorem source_reaches_side_analyse_eff:
+  assumes dom:
+    "\<And>v. cfg_reaches g (cfg_entry g) v \<Longrightarrow>
+      side_cfg_solve_dom_eff g etf bot s0 gseed v"
+  shows "\<exists>v t stk.
+     concrete_program_match Pi ps main src' (v, t, stk) \<and>
+     t \<in> \<lbrakk>side_analyse_eff Pi ps main etf bot s0 gseed v\<rbrakk>"
+proof -
+  have tfm':
+      "threefold_mono (side_cfg_T_eff (compile_prog Pi ps main) etf bot s0 gseed)"
+    using tfm g_def by simp
+  have dom':
+      "\<And>v. cfg_reaches (compile_prog Pi ps main)
+            (cfg_entry (compile_prog Pi ps main)) v \<Longrightarrow>
+          side_cfg_solve_dom_eff
+            (compile_prog Pi ps main) etf bot s0 gseed v"
+    using dom g_def by simp
+  show ?thesis
+    by (rule concrete_source_reaches_side_analyse_eff[
+          OF wf run se tfm' cone init dom'])
+qed
+
+end
+
 
 end
